Pulled out some irrelevant content from the tank example

simplefmi/SimpleTank.thy
@@ -3,6 +3,7 @@ theory SimpleTank
     VDMRT
     SimpleFMI
     "../hybrid/utp_hybrid"
+    "../theories/utp_reactive_hoare"
 begin recall_syntax
   
 alphabet tank_st =
@@ -18,6 +19,10 @@ begin
   lift_definition open_tank_st_ext :: "'a tank_st_scheme set \<Rightarrow> bool" is "open" .
   instance by (intro_classes, (transfer, auto simp add: separation_t2)+)
 end
+
+lemma continuous_Rep_tank_st_ext [continuous_intros]:
+  "continuous_on UNIV Rep_tank_st_ext"
+  by (metis continuous_on_open_vimage image_vimage_eq open_Int open_UNIV open_tank_st_ext.rep_eq)
   
 alphabet ctr_st = vrt_st +
   valveOn     :: bool
@@ -48,9 +53,6 @@ abbreviation (input) tank_sol_1 :: "real \<Rightarrow> real \<Rightarrow> real" 
 
 abbreviation (input) tank_sol_2 :: "real \<Rightarrow> real \<Rightarrow> real" where
 "tank_sol_2 \<equiv> (\<lambda> l\<^sub>0 t. l\<^sub>0 - t)"
-
-method linear_ode = 
-  (rule_tac uos_impl_uniq_sol[where L=1], (unfold_locales, auto intro!: continuous_on_Pair continuous_on_const Topological_Spaces.continuous_on_fst Topological_Spaces.continuous_on_snd continuous_on_snd simp add: lipschitz_def dist_Pair_Pair prod.case_eq_if)[1], (auto)[1], ode_cert)  
   
 lemma tank_ode_usol_1:
   "l > 0 \<Longrightarrow> (tank_sol_1 l\<^sub>0 usolves_ode tank_ode_1 from 0) {0..l} UNIV"
@@ -61,9 +63,9 @@ lemma tank_ode_usol_2:
   by (linear_ode)
     
 definition Tank  :: "real \<Rightarrow> tank_st trel" where 
-  "Tank area = H2T((\<langle>{&level} \<bullet> tank_ode_1(ti)\<rangle>\<^sub>h \<and> level \<leftarrow>\<^sub>h $level) 
+  "Tank area = H2T((\<langle>{&level} : tank_ode_1(ti)\<rangle>\<^sub>h \<and> level \<leftarrow>\<^sub>h $level) 
                      \<triangleleft> &valve \<triangleright>\<^sub>h 
-                   (\<langle>{&level} \<bullet> tank_ode_2(ti)\<rangle>\<^sub>h \<and> level \<leftarrow>\<^sub>h $level))"
+                   (\<langle>{&level} : tank_ode_2(ti)\<rangle>\<^sub>h \<and> level \<leftarrow>\<^sub>h $level))"
 
 definition Ctr :: "real \<Rightarrow> real \<Rightarrow> ctr_st vrel" where
 "Ctr minLevel maxLevel = 
@@ -74,31 +76,9 @@ definition
   "WaterTank minLevel maxLevel area = 
      FMI Init [FMU[ctr, Ctr minLevel maxLevel], FMU[tank, Tank area]] ArbStep Wiring"
 
-lift_definition var_all_res :: "'\<alpha> upred \<Rightarrow> ('a \<Longrightarrow> '\<alpha>) \<Rightarrow> '\<alpha> upred" is
-"\<lambda> P x b. \<forall> b'. P (b' \<oplus>\<^sub>L b on x)" .
-
-syntax
-  "_uvar_all_res" :: "logic \<Rightarrow> salpha \<Rightarrow> logic" (infixl "\<restriction>\<^sub>\<forall>" 90)
-    
-translations
-  "_uvar_all_res P x b" == "CONST var_all_res P x b"
-  
-definition pred_ares :: "'\<alpha> upred \<Rightarrow> ('\<beta> \<Longrightarrow> '\<alpha>) \<Rightarrow> '\<beta> upred" 
-  where [upred_defs]: "pred_ares P a = (P \<restriction>\<^sub>v a) \<restriction>\<^sub>p a"
-    
-
-update_uexpr_rep_eq_thms
-    
-syntax
-  "_pred_ares" :: "logic \<Rightarrow> salpha \<Rightarrow> logic" (infixl "\<restriction>\<^sub>q" 90)
-
-translations
-  "_pred_ares P a" == "CONST pred_ares P a"
-  
-thm "des_vars.defs"
-    
+        
 lemma fmu_hoare_rp [hoare_safe]:
-  "\<lbrakk> x \<natural> p; \<lbrace>p\<restriction>\<^sub>qx\<rbrace>Q\<lbrace>p\<restriction>\<^sub>qx\<rbrace>\<^sub>r \<rbrakk> \<Longrightarrow> \<lbrace>p\<rbrace>FMU[x, Q]\<lbrace>p\<rbrace>\<^sub>r"
+  "\<lbrakk> x \<natural> p; \<lbrace>p\<restriction>\<^sub>px\<rbrace>Q\<lbrace>p\<restriction>\<^sub>px\<rbrace>\<^sub>r \<rbrakk> \<Longrightarrow> \<lbrace>p\<rbrace>FMU[x, Q]\<lbrace>p\<rbrace>\<^sub>r"
   apply (rel_simp, auto simp add: des_vars.defs rp_vars.defs)
   apply (rename_tac ok wait tr st ok' wait' tr' st')
   apply (drule_tac x="ok" in spec)
@@ -111,131 +91,27 @@ lemma fmu_hoare_rp [hoare_safe]:
   apply (drule_tac x="get\<^bsub>x\<^esub> st'" in spec)
   apply (auto)
 done
-        
-method ode_solve 
-  for sol :: "'a::ordered_euclidean_space \<Rightarrow> real \<Rightarrow> 'a" 
-  = (rule_tac trans, rule_tac ode_solution'[where \<F> = "sol"], simp_all, linear_ode, rel_auto)
-    
+  
 lemma tank_ode_1_evolve:
-  "\<langle>&level \<bullet> tank_ode_1(ti)\<rangle>\<^sub>h = level \<leftarrow>\<^sub>h ($level + \<guillemotleft>ti\<guillemotright>)"
-  by (ode_solve tank_sol_1)
+  "\<langle>{&level} : tank_ode_1(ti)\<rangle>\<^sub>h = {[&level \<mapsto>\<^sub>s \<guillemotleft>op +\<guillemotright>(&level)\<^sub>a(\<guillemotleft>ti\<guillemotright>)\<^sub>a]}\<^sub>h"
+  by (ode_fsolve tank_sol_1)
 
 lemma tank_ode_2_evolve:
-  "\<langle>&level \<bullet> tank_ode_2(ti)\<rangle>\<^sub>h = level \<leftarrow>\<^sub>h ($level - \<guillemotleft>ti\<guillemotright>)"
-  by (ode_solve tank_sol_2)
+  "\<langle>{&level} : tank_ode_2(ti)\<rangle>\<^sub>h = {[&level \<mapsto>\<^sub>s \<guillemotleft>op -\<guillemotright>(&level)\<^sub>a(\<guillemotleft>ti\<guillemotright>)\<^sub>a]}\<^sub>h"
+  by (ode_fsolve tank_sol_2) 
     
-definition hFrame :: "('a \<Longrightarrow> 'c::t2_space) \<Rightarrow> ('d, 'c) hyrel \<Rightarrow> ('d, 'c) hyrel" where
-[upred_defs]: "hFrame x P = (P \<and> \<lceil>x:[true]\<rceil>\<^sub>h)"
-  
-syntax
-  "_hFrame" :: "salpha \<Rightarrow> logic \<Rightarrow> logic" ("_:[_]\<^sub>h" [99,0] 100)
-
-translations
-  "_hFrame a P" == "CONST hFrame a P"
-  
-abbreviation hODE_frame ::
-  "('a::ordered_euclidean_space \<Longrightarrow> 'c::t2_space) \<Rightarrow>
-   'a ODE \<Rightarrow> ('d, 'c) hyrel" where
-"hODE_frame x \<F>' \<equiv> hFrame x (hODE x \<F>')"
-        
-syntax
-  "_hODE_frame" :: "salpha \<Rightarrow> logic \<Rightarrow> logic" ("\<langle>_ : _\<rangle>\<^sub>h")
-
-translations
-  "_hODE_frame a P" => "CONST hODE_frame a (\<lambda> _time_var. P)"
-  "_hODE_frame a P" <= "CONST hODE_frame a (\<lambda> t. P)"    
-  
-definition hEvolves :: "(real \<Rightarrow> 'c::t2_space usubst) \<Rightarrow> ('d, 'c) hyrel" where
-[upred_defs]: "hEvolves s = (\<lceil>\<langle>s(ti)\<rangle>\<^sub>a\<rceil>\<^sub>h \<and> \<^bold>l >\<^sub>u 0)"
-    
-syntax
-  "_hEvolves" :: "logic \<Rightarrow> logic" ("{_}\<^sub>h")
-
-translations
-  "_hEvolves s" => "CONST hEvolves (\<lambda> _time_var. s)"
-  "_hEvolves s" <= "CONST hEvolves (\<lambda> t. s)"
-  
-lemma hEvolves_id: 
-  "{id}\<^sub>h = \<^bold>v \<leftarrow>\<^sub>h $\<^bold>v"
-  by (rel_auto)
-
-thm ode_solution
-      
-theorem ode_frame_solution:
-  assumes 
-    "vwb_lens x" "\<forall> x. \<forall> l > 0. (\<F>(x) usolves_ode \<F>' from 0) {0..l} UNIV" "\<forall> x. \<F>(x)(0) = x"
-  shows "\<langle>x : \<F>'(ti)\<rangle>\<^sub>h = {[x \<mapsto>\<^sub>s \<guillemotleft>\<F>\<guillemotright>(&x)\<^sub>a(\<guillemotleft>ti\<guillemotright>)\<^sub>a]}\<^sub>h"
-proof -
-  have "\<langle>x : \<F>'(ti)\<rangle>\<^sub>h = x:[x \<leftarrow>\<^sub>h \<guillemotleft>\<F>\<guillemotright>($x)\<^sub>a(\<guillemotleft>ti\<guillemotright>)\<^sub>a]\<^sub>h"
-    by (simp add: ode_solution[where \<F>=\<F>] assms)
-  also from assms(1) have "... = (\<lceil>$x\<acute> =\<^sub>u \<guillemotleft>\<F>\<guillemotright>($x)\<^sub>a(\<guillemotleft>ti\<guillemotright>)\<^sub>a \<and> x:[true]\<rceil>\<^sub>h \<and> 0 <\<^sub>u \<^bold>l)"
-    by (rel_auto)
-  also from assms(1) have "... = (\<lceil>x:[$x\<acute> =\<^sub>u \<guillemotleft>\<F>\<guillemotright>($x)\<^sub>a(\<guillemotleft>ti\<guillemotright>)\<^sub>a]\<rceil>\<^sub>h \<and> 0 <\<^sub>u \<^bold>l)"      
-    by (simp add: antiframe_conj_true unrest)
-  also have "... = (\<lceil>x:[$x\<acute> =\<^sub>u \<lceil>\<guillemotleft>\<F>\<guillemotright>(&x)\<^sub>a(\<guillemotleft>ti\<guillemotright>)\<^sub>a\<rceil>\<^sub><]\<rceil>\<^sub>h \<and> 0 <\<^sub>u \<^bold>l)"
-    by (rel_auto)
-  also from assms(1) have "... = {[x \<mapsto>\<^sub>s \<guillemotleft>\<F>\<guillemotright>(&x)\<^sub>a(\<guillemotleft>ti\<guillemotright>)\<^sub>a]}\<^sub>h"
-    by (simp add: antiframe_assign hEvolves_def, rel_auto)
-  finally show ?thesis .
-qed
-  
-lemma hyrel2trel_hEvolves:
-  fixes x :: "'a::t2_space \<Longrightarrow> 'c::t2_space"
-  assumes "continuous_lens x" "continuous_on {0..} f"
-  shows "H2T({[x \<mapsto>\<^sub>s \<guillemotleft>f(ti)\<guillemotright>]}\<^sub>h) = 
-         (\<Sqinter> t | \<guillemotleft>t\<guillemotright> >\<^sub>u 0 \<bullet> wait\<^sub>r(\<guillemotleft>t\<guillemotright>) ;; x :=\<^sub>r \<guillemotleft>f(real_of_pos t)\<guillemotright>)" (is "?lhs = ?rhs")
-proof -
-  from assms(1) 
-  have "?lhs = R1 (\<^bold>\<exists> l \<bullet> ({[x \<mapsto>\<^sub>s \<guillemotleft>f ti\<guillemotright>]}\<^sub>h \<and> end\<^sub>u(&tt) =\<^sub>u \<guillemotleft>l\<guillemotright> \<and> rl(&\<^bold>v) \<and> $st:\<^bold>d\<acute> =\<^sub>u $st:\<^bold>d :: (unit,'c) hyrel)  \<restriction>\<^sub>r &st:\<^bold>c \<oplus>\<^sub>r st \<and> &tt =\<^sub>u \<guillemotleft>mk_pos l\<guillemotright>)"
-    by (simp add: hyrel2trel_def)
-  also have "... = R1(\<^bold>\<exists> l \<bullet> ((x := \<guillemotleft>f(l)\<guillemotright>) \<oplus>\<^sub>r st) \<and> \<guillemotleft>l\<guillemotright> >\<^sub>u 0 \<and> &tt =\<^sub>u \<guillemotleft>mk_pos l\<guillemotright>)" (is "?P = ?Q")
-  proof (rule antisym)
-    show "?P \<sqsubseteq> ?Q"
-      apply (rel_simp)
-      apply (rename_tac tr st tr' n)
-      apply (rule_tac x="n" in exI)
-      apply (auto)
-      apply (rule_tac x="0" in exI)
-      apply (rule_tac x="tt_mk n (\<lambda> t. put\<^bsub>x\<^esub> st (f t))" in exI)
-      apply (subgoal_tac "continuous_on {0..n} (put\<^bsub>x\<^esub> st \<circ> f)")
-       apply (auto simp add: assms Limit_solve at_left_from_zero)[1]
-       apply (rule continuous_on_compose)
-       apply (meson Icc_subset_Ici_iff assms continuous_on_subset order_refl)
-        apply (rule continuous_lens.put_continuous_v[OF assms(1)])
-    done
-    show "?Q \<sqsubseteq> ?P"
-      apply (rel_simp)
-      apply (rename_tac tr tr' tr'' tr''')
-      apply (rule_tac x="end\<^sub>t (tr''' - tr'')" in exI)
-      apply (auto)
-       apply (subst Limit_solve_at_left)
-          apply (auto)
-       apply (subgoal_tac "continuous_on {0..end\<^sub>t (tr''' - tr'')} (put\<^bsub>x\<^esub> tr \<circ> f)")
-        apply (simp)
-       apply (rule continuous_on_compose)
-       apply (meson Icc_subset_Ici_iff assms continuous_on_subset order_refl)
-       apply (rule continuous_lens.put_continuous_v[OF assms(1)])
-    done
-  qed
-  also have "... = ?rhs"
-    apply (rel_auto)
-    apply (metis le_add_diff_inverse less_eq_real_def mk_pos_less mk_pos_zero real_of_pos)
-    apply (metis (full_types) approximation_preproc_push_neg(3) least_zero mk_pos.abs_eq mk_pos_real_of_pos not_le zero_pos.abs_eq)
-  done
-  finally show ?thesis .
-qed
-
-      
-    
-term "[$level \<mapsto>\<^sub>s $x]"
+lemma continuous_lens_level [closure]: "continuous_lens level"
+  apply (unfold_locales, simp_all add: lens_defs prod.case_eq_if)
+  apply (simp add: tank_st.select_defs iso_tuple_fst_def tuple_iso_tuple_def 
+      tank_st_ext_Tuple_Iso_def Topological_Spaces.continuous_on_fst continuous_Rep_tank_st_ext)
+  sorry
     
     
-lemma "(\<Sigma> :: tank_st \<Longrightarrow> tank_st) \<approx>\<^sub>L level +\<^sub>L valve"
-    
-    
-lemma "H2T(\<langle>&level \<bullet> \<lambda>lev. 1\<rangle>\<^sub>h \<triangleleft> &valve \<triangleright>\<^sub>h \<langle>&level \<bullet> \<lambda>lev. - 1\<rangle>\<^sub>h) = undefined"
-  apply (simp add: hyrel2trl_cond hyrel2trel_hEvolve tank_ode_1_evolve tank_ode_2_evolve)
-  thm hyrel2trel_hEvolve
+lemma "H2T(\<langle>&level : \<lambda>lev. 1\<rangle>\<^sub>h \<triangleleft> &valve \<triangleright>\<^sub>h \<langle>&level : \<lambda>lev. - 1\<rangle>\<^sub>h) = undefined"
+  apply (simp add: hyrel2trl_cond hyrel2trel_hEvolves tank_ode_1_evolve tank_ode_2_evolve closure)
+  thm hyrel2trel_hEvolves
+    thm hyrel2trel_hEvolves
+  apply (subst hyrel2trel_hEvolves)
     
 lemma "\<lbrace>true\<rbrace>WaterTank 0 10 10\<lbrace>&tank:level <\<^sub>u 10 \<and> &ctr:levelSensor <\<^sub>u 10\<rbrace>\<^sub>r"
   apply (simp add: conj_comm conj_assoc)
